---
title: 'DATA 605 HW14'
author: "Josh Iden"
date: "`r Sys.Date()`"
output:
  prettydoc::html_pretty:
    theme: cayman
    highlight: github
    math: katex
---

```{r setup, include=FALSE}
knitr::opts_chunk$set(echo = TRUE)
library(pracma)
```

![](/Users/joshiden/Documents/Classes/CUNY%20SPS/Fall%202022/DATA%20605%20/HW/DATA-605/HW/HW14/DATA605_HW14.png)

----

# Q1:

$$f(x) = 1-x$$  

----

The Taylor series $f(x)$ at $a$ is defined as:

$f(x) = f(a) + \frac{f'(a)}{1!}(x-a) + \frac{f''(a)}{2!}(x -a)^2 + \frac{f'''(a)}{3!}(x-a)^3 + ...$

With a center 0: 1-x

$= 1 + \frac{f'(1-x)(0)}{1!}x + \frac{f''(1-x)(0)}{2!}x^2 + \frac{f'''(1-x)(0)}{3!}x^3 + ...$

$= 1 + \frac{-1}{1!}x + \frac{0}{2!}x^2 + \frac{0}{3!}x^3 + \frac{0}{4!}x^4 + \frac{0}{5!}x^5 + ...$

$= 1-x$

```{r}
f1 = function(x){
  1-x
}
taylor(f1, 0, 5)

```

----

# Q2:

$$f(x) = e^x$$\

----  

The derivative of $e^x$ is always $e^x$  

so,

$= 1 + \frac{f'x(e^x)(0)}{1!}x + \frac{f''(e^x)(0)}{2!}x^2 + \frac{f'''(e^x)(0)}{3!}x^3 + ...$

$= 1 + \frac{1}{1!}x + \frac{1}{2!}x^2 + \frac{1}{3!}x^3 + \frac{1}{4!}x^4 + ...$

The series sum representation is:

$\sum^{\infty}_{n=0}\frac{x^n}{n!}$

```{r}
f2 = function(x) {
  exp(x)
}

taylor(f2,0,4)

```

----

# Q3:

$$f(x) = ln(1 + x)$$  

----

$= 0 + \frac{f'x(ln(1+x))(0)}{1!}x + \frac{f''(ln(1+x))(0)}{2!}x^2 + \frac{f'''(ln(1+x))(0)}{3!}x^3 + ...$

$= 0 + \frac{1}{1!}x + \frac{-1}{2!}x^2 + \frac{2}{3!}x^3 + \frac{-6}{4!}x^4 + \frac{24}{5!}x^5 + ...$

\$= x - \frac{1}{2}x\^2 + \frac{1}{3}x\^3 - \frac{1}{4}x\^4 + \frac{1}{5}x\^5 + ... \$

The sum series representation is:

$\sum^{\infty}_{n=1}(-1)^{n+1}\frac{x^n}{n}$

```{r}
f3 = function(x) {
  log(1+x)
}

taylor(f3, 0, 5)
```

------------------------------------------------------------------------

# Q4:

$$f(x) = x^{\frac{1}{2}}$$

------------------------------------------------------------------------

$= 1 + \frac{f'x(x^{\frac{1}{2}})(1)}{1!}(x - 1) + \frac{f''(x^{\frac{1}{2}})(1)}{2!}(x-1)^2 + \frac{f'''(x^{\frac{1}{2}})(1)}{3!}(x-1)^3 + ...$

$= 1 + \frac{{\frac{1}{2}}}{1!}(x - 1) + \frac{-{\frac{1}{4}}}{2!}(x-1)^2 + \frac{{\frac{3}{8}}}{3!}(x-1)^3 + \frac{-{\frac{15}{16}}}{4!}(x-1)^4 ...$

$= 1 + \frac{1}{2}(x-1) - \frac{1}{8}(x-1)^2 + \frac{1}{16}(x-1)^3 - \frac{5}{128}(x-1)^4 + ...$

Thus, the Taylor series $x^{\frac{1}{2}}$ with center 1 $= 1 + \frac{1}{2}(x-1) - \frac{1}{8}(x-1)^2 + \frac{1}{16}(x-1)^3 - \frac{5}{128}(x-1)^4 + ...$
